theories/Semantics.v
@@ -5,8 +5,8 @@ From Stdlib Require Import ZArith.ZArith.
 
 From stdpp Require Import gmap.
 From stdpp Require Import relations.
+From stdpp Require Import tactics.
 
-From RSL Require Import Tactics.
 From RSL Require Import RTL.
 From RSL Require Import Notations.
 
@@ -26,24 +26,24 @@ Definition val_to_loc (v: val) : option loc :=
   then Some (Z.to_pos v)
   else None.
 
-Definition get_reg (ρ: regmap) (r: reg) : val :=
+Definition get_reg (r: reg) (ρ: regmap) : val :=
   match ρ !! r with
   | Some v => v
   | None => 0%Z (* Dummy val *)
   end.
 
-Definition get_regs (ρ: regmap) (l: list reg) : list val :=
-  map (fun r => get_reg ρ r) l.
+Definition get_regs (l: list reg) (ρ: regmap) : list val :=
+  map (fun r => get_reg r ρ) l.
 
-Definition set_reg (ρ: regmap) (r: reg) (v: val) : regmap := <[r := v]>ρ.
+Definition set_reg (r: reg) (v: val) (ρ: regmap) : regmap := <[r := v]>ρ.
 
-Definition get_at (m: memory) (addr: val) : option val :=
+Definition get_at (addr: val) (m: memory) : option val :=
   match val_to_loc addr with
   | Some loc => m !! loc
   | None => None
   end.
 
-Definition update_at (m: memory) (addr: val) (f: val -> val) : option memory
+Definition update_at (addr: val) (f: val -> val) (m: memory) : option memory
   := match val_to_loc addr with
      | Some loc =>
          match m !! loc with
@@ -53,8 +53,8 @@ Definition update_at (m: memory) (addr: val) (f: val -> val) : option memory
      | None => None
      end.
 
-Definition set_at (m: memory) (addr: val) (v: val) : option memory :=
-  update_at m addr (fun _ => v).
+Definition set_at (addr: val) (v: val) (m: memory) : option memory :=
+  update_at addr (fun _ => v) m.
 
 (* Assert that instruction at [pc] in function [f] is [i] *)
 Notation "f '@' pc 'is' i" :=
@@ -109,32 +109,32 @@ Inductive step (P: program) : state -> state -> Prop :=
 
 | exec_Iret: forall σ m ρ f pc r v,
   f@pc is <{ ret r }> ->
-  get_reg ρ r = v ->
+  get_reg r ρ = v ->
   P |- (σ, State f pc ρ, m) ->> (σ, ReturnState v, m)
 
 | exec_Iop: forall σ m ρ f pc op args dst pc' ρ' v,
   f@pc is <{ dst := @op args -> pc' }> ->
-  eval_op op (get_regs ρ args) = Some v ->
-  set_reg ρ dst v = ρ' ->
+  eval_op op (get_regs args ρ) = Some v ->
+  set_reg dst v ρ = ρ' ->
   P |- (σ, State f pc ρ, m) ->> (σ, State f pc' ρ', m)
 
 | exec_Iload: forall σ m ρ f pc dst src pc' ρ' addr v,
   f@pc is <{ dst := !src -> pc' }> ->
-  get_reg ρ src = addr ->
-  get_at m addr = Some v ->
-  set_reg ρ dst v = ρ' ->
+  get_reg src ρ = addr ->
+  get_at addr m = Some v ->
+  set_reg dst v ρ = ρ' ->
   P |- (σ, State f pc ρ, m) ->> (σ, State f pc' ρ', m)
 
 | exec_Istore: forall σ m ρ f pc dst src pc' m' addr v,
   f@pc is <{ !dst := src -> pc' }> ->
-  get_reg ρ dst = addr ->
-  get_reg ρ src = v ->
-  set_at m addr v = Some m' ->
+  get_reg dst ρ = addr ->
+  get_reg src ρ = v ->
+  set_at addr v m = Some m' ->
   P |- (σ, State f pc ρ, m) ->> (σ, State f pc' ρ, m')
 
 | exec_Icond: forall  σ m ρ f pc cond ifso ifnot v pc',
   f@pc is <{ if cond then goto ifso else goto ifnot }> ->
-  get_reg ρ cond = v ->
+  get_reg cond ρ = v ->
   pc' = (if Z.eqb v 0 then ifso else ifnot) ->
   P |- (σ, State f pc ρ, m) ->> (σ, State f pc' ρ, m)
 
@@ -142,14 +142,15 @@ Inductive step (P: program) : state -> state -> Prop :=
   f@pc is <{ dst := @call sig args -> pc' }> ->
   find_fun P sig = Some fn ->
   Stackframe dst f pc' ρ :: σ = σ' ->
-  P |- (σ, State f pc ρ, m) ->> (σ', CallState fn (get_regs ρ args), m)
+  P |- (σ, State f pc ρ, m) ->> (σ', CallState fn (get_regs args ρ), m)
 
 | exec_function: forall σ m ρ f args,
-  init_regs args (in_regs f.(fn_sig)) = ρ ->
+  length args = length (fn_regs f) ->
+  init_regs args (fn_regs f) = ρ ->
   P |- (σ, CallState f args, m) ->> (σ, State f (fn_entrypoint f) ρ, m)
 
 | exec_return: forall σ m ρ f pc dst v ρ',
-  set_reg ρ dst v = ρ' ->
+  set_reg dst v ρ = ρ' ->
   P |- (Stackframe dst f pc ρ :: σ, ReturnState v, m) ->> (σ, State f pc ρ', m)
 
 where "P '|-' s '->>' t" := (step P s t).
@@ -231,7 +232,7 @@ Lemma unfold_call P fn : ∀ n res f pc ρ args m σ t m',
     (∃ m1 m2 v m'',
         n = 1 + m1 + m2
         ∧ P |- ([], CallState fn args, m) -{m1}> ([], ReturnState v, m'')
-        ∧ P |- ([], State f pc (set_reg ρ res v), m'') -{m2}> (σ, t, m')
+        ∧ P |- ([], State f pc (set_reg res v ρ), m'') -{m2}> (σ, t, m')
     ).
 Proof.
   intros n.
@@ -242,13 +243,13 @@ Proof.
     apply IH in Hrtc.
     destruct Hrtc
       as [(σ' & -> & Hlift) | (m1 & m2 & v & m'' & Hn & Hcall & Hrest)].
-    + inv Hstep;
+    + inv Hstep as [ | | | | | | | | ? ? ? ? ? ? v ? ? Hσ];
         try (left; eexists; split;
              [ rewrite ? app_comm_cons; reflexivity
              | eapply nsteps_r; [ now apply Hlift | econstructor; now eauto]
              ]
           ).
-      destruct σ'; inv H.
+      destruct σ'; inv Hσ.
       * right. exists n, 0, v, m'. repeat split; eauto. constructor.
       * left. eexists. split.
         -- reflexivity.
@@ -257,3 +258,57 @@ Proof.
         now eauto || (eapply nsteps_r;
                       [ now apply Hrest | econstructor; now eauto]).
 Qed.
+
+Lemma get_regs_insert : ∀ regs r v ρ,
+  r ∉ regs ->
+  get_regs regs (<[r := v]> ρ) = get_regs regs ρ.
+Proof.
+  intros regs r v ρ.
+  induction regs as [|r' regs' IH]; intros Hnotin; [reflexivity |].
+  simpl. f_equal.
+  - unfold get_reg. rewrite (lookup_insert_ne ρ); set_solver.
+  - apply IH. set_solver.
+Qed.
+
+Lemma get_regs_init_regs : ∀ regs args,
+  NoDup regs ->
+  length args = length regs ->
+  get_regs regs (init_regs args regs) = args.
+Proof.
+  intros regs args Hnodup.
+  revert args.
+  induction Hnodup as [|r regs Hnotin Hnodup IH]; intros args Hlen.
+  - destruct args; [reflexivity | discriminate Hlen].
+  - destruct args as [|v args]; [discriminate Hlen |].
+    simpl in Hlen. injection Hlen as Hlen'.
+    simpl. f_equal.
+    + unfold get_reg. now rewrite (lookup_insert_eq (init_regs args regs)).
+    + rewrite get_regs_insert by exact Hnotin.
+      apply IH. exact Hlen'.
+Qed.
+
+Lemma get_reg_set_reg_eq : ∀ r v ρ,
+  get_reg r (set_reg r v ρ) = v.
+Proof.
+  intros r v ρ.
+  unfold get_reg, set_reg.
+  now rewrite (lookup_insert_eq ρ).
+Qed.
+
+Lemma get_reg_set_reg_neq : ∀ r r' v ρ,
+  r ≠ r' -> get_reg r (set_reg r' v ρ) = get_reg r ρ.
+Proof.
+  intros r r' v ρ Hneq.
+  unfold get_reg, set_reg.
+  now rewrite (lookup_insert_ne ρ).
+Qed.
+
+Tactic Notation "simpl_reg" "by" tactic3(tac) :=
+  repeat match goal with
+    | _ => progress tac
+    | |- context[get_reg _ (set_reg _ _ _)] =>
+        (rewrite get_reg_set_reg_neq by tac)
+        || (rewrite get_reg_set_reg_eq by tac)
+    end.
+
+Tactic Notation "simpl_reg" := simpl_reg by (f_equal; lia).
